Computability/Constructions/Primitive.lean
@@ -471,3 +471,84 @@ theorem c_ef_ev_left (h:(eval O c x).Dom) : eval O (left.comp $ c_ef c) x = x :=
   simp [Seq.seq]
   exact Part.Dom.bind h fun y ↦ Part.some x
 end ef
+
+
+section nat_iterate
+namespace Nat.RecursiveIn.Code
+def c_nat_iterate (cf:Code) :=
+  prec
+  c_id
+  (cf.comp (right.comp right))
+
+@[simp] theorem c_nat_iterate_ev_pr (hcf:code_prim cf) : code_prim (c_nat_iterate cf) := by unfold c_nat_iterate; repeat (first|assumption|simp|constructor)
+@[simp] theorem c_nat_iterate_evp : eval_prim O (c_nat_iterate cf) (Nat.pair input i) = (eval_prim O cf)^[i] (input) := by
+  simp [c_nat_iterate]
+  induction i with
+  | zero => simp
+  | succ n ih =>
+    simp [ih]
+    exact Eq.symm (Function.iterate_succ_apply' (eval_prim O cf) n input)
+-- @[simp] theorem c_nat_iterate_ev :eval O (c_nat_iterate cf) (Nat.pair input i) = (eval_prim O cf)^[i] (input) := by
+--     simp [← eval_prim_eq_eval c_nat_iterate_ev_pr]
+end Nat.RecursiveIn.Code
+end nat_iterate
+
+
+
+
+
+section mul2
+namespace Nat.RecursiveIn.Code
+def c_mul2 := c_mul.comp₂ c_id (c_const 2)
+@[simp] theorem c_mul2_ev_pr:code_prim c_mul2 := by unfold c_mul2; repeat (first|assumption|simp|constructor)
+@[simp] theorem c_mul2_evp:eval_prim O c_mul2 = fun x => x*2 := by simp [c_mul2]
+@[simp] theorem c_mul2_ev:eval O c_mul2 = (fun x => x*(2:ℕ)) := by rw [← eval_prim_eq_eval c_mul2_ev_pr]; simp only [c_mul2_evp];
+end Nat.RecursiveIn.Code
+-- theorem Nat.PrimrecIn.mul2:Nat.PrimrecIn O Nat.mul2 := by ...
+-- theorem Nat.Primrec.mul2:Nat.Primrec Nat.mul2 := by ...
+end mul2
+
+
+
+namespace Nat.RecursiveIn.Code
+def c_pair := c_add.comp₂ (c_mul2.comp $ c_mul2) (c_const 5)
+@[simp, aesop safe] theorem c_pair_ev_pr:code_prim c_pair := by unfold c_pair; repeat (first|assumption|simp|constructor)
+@[simp] theorem c_pair_evp : eval_prim O c_pair (Nat.pair a b) = encodeCode (pair a b) := by simp [encodeCode, c_pair, Nat.mul_comm]
+@[simp] theorem c_pair_ev:eval O c_pair (Nat.pair a b) = encodeCode (pair a b) := by rw [← eval_prim_eq_eval c_pair_ev_pr]; simp
+
+def c_comp := c_add.comp₂ (c_mul2.comp $ c_mul2) (c_const 6)
+@[simp, aesop safe] theorem c_comp_ev_pr:code_prim c_comp := by unfold c_comp; repeat (first|assumption|simp|constructor)
+@[simp] theorem c_comp_evp : eval_prim O c_comp (Nat.pair a b) = encodeCode (comp a b) := by simp [encodeCode, c_comp, Nat.mul_comm]
+@[simp] theorem c_comp_ev:eval O c_comp (Nat.pair a b) = encodeCode (comp a b) := by rw [← eval_prim_eq_eval c_comp_ev_pr]; simp
+
+def c_prec := c_add.comp₂ (c_mul2.comp $ c_mul2) (c_const 7)
+@[simp, aesop safe] theorem c_prec_ev_pr:code_prim c_prec := by unfold c_prec; repeat (first|assumption|simp|constructor)
+@[simp] theorem c_prec_evp : eval_prim O c_prec (Nat.pair a b) = encodeCode (prec a b) := by simp [encodeCode, c_prec, Nat.mul_comm]; exact rfl
+@[simp] theorem c_prec_ev:eval O c_prec (Nat.pair a b) = encodeCode (prec a b) := by rw [← eval_prim_eq_eval c_prec_ev_pr]; simp
+
+def c_rfind' := c_add.comp₂ (c_mul2.comp $ c_mul2) (c_const 8)
+@[simp, aesop safe] theorem c_rfind'_ev_pr:code_prim c_rfind' := by unfold c_rfind'; repeat (first|assumption|simp|constructor)
+@[simp] theorem c_rfind'_evp : eval_prim O c_rfind' c = encodeCode (rfind' c) := by simp [encodeCode, c_rfind', Nat.mul_comm]; exact rfl
+@[simp] theorem c_rfind'_ev:eval O c_rfind' c = encodeCode (rfind' c) := by rw [← eval_prim_eq_eval c_rfind'_ev_pr]; simp
+
+def c_c_const := (c_nat_iterate (c_comp.comp₂ (c_const succ) (c_id))).comp₂ zero c_id
+@[simp, aesop safe] theorem c_c_const_ev_pr:code_prim c_c_const := by unfold c_c_const; repeat (first|assumption|simp|constructor)
+@[simp] theorem c_c_const_evp : eval_prim O c_c_const n = encodeCode (c_const n) := by
+  unfold c_const
+  unfold c_c_const
+  simp
+  induction n with
+  | zero => simp [encodeCode]
+  | succ n ih =>
+    simp [Function.iterate_succ', -Function.iterate_succ]
+    rw [ih]
+    apply Eq.symm
+    rw [c_const.eq_def] -- bug? cant rw without the eq.symm, even with occs
+    simp only [decodeCode_encodeCode]
+@[simp] theorem c_c_const_ev:eval O c_c_const c = encodeCode (c_const c) := by rw [← eval_prim_eq_eval c_c_const_ev_pr]; simp
+
+def c_ev_const := c_comp.comp₂ left (c_c_const.comp right)
+@[simp, aesop safe] theorem c_ev_const_ev_pr:code_prim c_ev_const := by unfold c_ev_const; repeat (first|assumption|simp|constructor)
+@[simp] theorem c_ev_const_evp : eval_prim O c_ev_const (Nat.pair e x) = encodeCode (comp e (c_const x)) := by simp [c_ev_const]
+@[simp] theorem c_ev_const_ev:eval O c_ev_const (Nat.pair e x) = encodeCode (comp e (c_const x)) := by rw [← eval_prim_eq_eval c_ev_const_ev_pr]; simp
+end Nat.RecursiveIn.Code
